Implement and test delay with clock enable

tests/TestsSV.hs
@@ -29,6 +29,8 @@ main = do writeSystemVerilog instantiateNetlist
           writeTestBench mult2_3_5_tb
           writeSystemVerilog delayByte_Netlist
           writeTestBench delayByte_tb
+          writeSystemVerilog delayEnableByte_Netlist
+          writeTestBench delayEnableByte_tb
           writeSystemVerilog pipelinedNANDNetlist
           -- writeTestBench pipelinedNAND_tb
           writeSystemVerilog countBy_Netlist
